yjs/content.go
@@ -1,14 +1,14 @@
 package yjs
 
-// Content is the payload of an item. The Phase-1 simplification fixes this to a
+// content is the payload of an item. The Phase-1 simplification fixes this to a
 // single string type (y-octo's codec/content.rs has many variants).
 //
 // TODO: support more types
-type Content struct {
+type content struct {
 	content string
 }
 
-// Len is the number of clocks the content occupies (y-octo: Content::clock_len).
-func (c Content) Len() uint64 {
+// Len is the number of clocks the content occupies (y-octo: content::clock_len).
+func (c content) Len() uint64 {
 	return uint64(len(c.content))
 }
