yjs/refs.go
@@ -1,48 +1,48 @@
 package yjs
 
-// NodeLen is the (id, len) summary carried by GC and Skip nodes
-// (y-octo: codec/refs.rs NodeLen).
-type NodeLen struct {
-	id  Id
+// nodeLen is the (id, len) summary carried by GC and Skip nodes
+// (y-octo: codec/refs.rs nodeLen).
+type nodeLen struct {
+	id  id
 	len uint64
 }
 
-// Node is a struct-store entry: an Item, or a GC / Skip tombstone
-// (y-octo: codec/refs.rs Node).
-type Node interface {
+// node is a struct-store entry: an item, or a GC / Skip tombstone
+// (y-octo: codec/refs.rs node).
+type node interface {
 	isNode()
 	// nodeId is the start id of the run this node represents.
-	nodeId() Id
+	nodeId() id
 	// clock is the clock component of nodeId (start of the run).
 	clock() Clock
 	// length is the number of clocks this node occupies.
 	length() uint64
 }
 
-type GCNode struct {
-	nodeLen NodeLen
+type gcNode struct {
+	nodeLen nodeLen
 }
 
-type SkipNode struct {
-	nodeLen NodeLen
+type skipNode struct {
+	nodeLen nodeLen
 }
 
-type ItemNode struct {
-	item Item
+type itemNode struct {
+	item item
 }
 
-func (GCNode) isNode() {}
+func (gcNode) isNode() {}
 
-func (SkipNode) isNode() {}
+func (skipNode) isNode() {}
 
-func (ItemNode) isNode() {}
+func (itemNode) isNode() {}
 
-func (n GCNode) nodeId() Id       { return n.nodeLen.id }
-func (n GCNode) clock() Clock     { return n.nodeLen.id.clock }
-func (n GCNode) length() uint64   { return n.nodeLen.len }
-func (n SkipNode) nodeId() Id     { return n.nodeLen.id }
-func (n SkipNode) clock() Clock   { return n.nodeLen.id.clock }
-func (n SkipNode) length() uint64 { return n.nodeLen.len }
-func (n ItemNode) nodeId() Id     { return n.item.id }
-func (n ItemNode) clock() Clock   { return n.item.id.clock }
-func (n ItemNode) length() uint64 { return n.item.Len() }
+func (n gcNode) nodeId() id       { return n.nodeLen.id }
+func (n gcNode) clock() Clock     { return n.nodeLen.id.clock }
+func (n gcNode) length() uint64   { return n.nodeLen.len }
+func (n skipNode) nodeId() id     { return n.nodeLen.id }
+func (n skipNode) clock() Clock   { return n.nodeLen.id.clock }
+func (n skipNode) length() uint64 { return n.nodeLen.len }
+func (n itemNode) nodeId() id     { return n.item.id }
+func (n itemNode) clock() Clock   { return n.item.id.clock }
+func (n itemNode) length() uint64 { return n.item.Len() }
